compose

BB.v
@@ -1,176 +1,422 @@
 From Coq Require Import Lists.List.
 Import ListNotations.
-From Coq Require Import Vectors.Fin.
+From Coq Require Import Arith Lia.
+
+Record Finnat (n : nat) : Set := mkFinnat {
+  finnat_val :> nat;
+  finnat_lt : finnat_val < n
+}.
+Arguments mkFinnat {n}.
+Arguments finnat_val {n}.
+Arguments finnat_lt {n}.
+
+Lemma Finnat_ext {n : nat} (a b : Finnat n) :
+  finnat_val a = finnat_val b -> a = b.
+Proof.
+  destruct a as [va Ha], b as [vb Hb]; simpl.
+  intros ->. f_equal. apply Peano_dec.le_unique.
+Qed.
+
+Definition Finnat_eq_dec {n : nat} (a b : Finnat n) : {a = b} + {a <> b}.
+Proof.
+  destruct (Nat.eq_dec (finnat_val a) (finnat_val b)) as [H | H].
+  - left. now apply Finnat_ext.
+  - right. intros He. apply H. now rewrite He.
+Defined.
+
+Definition fin0 {n : nat} : Finnat (S n) :=
+  {| finnat_val := 0; finnat_lt := Nat.lt_0_succ n |}.
 
 Inductive direction : Set := L | R.
 
-Record TM : Set := {
+(* Alphabet: Finnat (2 + k).  Value 0 is blank, and 1 is the default score state. *)
+Definition symbol (k : nat) : Set := Finnat (S (S k)).
+Definition blank {k : nat} : symbol k := fin0.
+Definition one   {k : nat} : symbol k :=
+  {| finnat_val := 1; finnat_lt := le_n_S 1 (S k) (le_n_S 0 k (Nat.le_0_l k)) |}.
+
+Lemma blank_neq_one {k : nat} : @blank k <> @one k .
+Proof.
+  intros H. discriminate.
+Qed.
+
+Record TM (k : nat) : Set := mkTM {
   number_of_states : nat;
-  state : Set := Fin.t number_of_states;
-  number_of_symbols : nat;
-  symbol : Set := Fin.t number_of_symbols;
-  blank_symbol : symbol;
-  transition_function : state -> symbol -> option (state * symbol * direction); 
-  start_state : state
+  transition_function :
+    Finnat number_of_states -> symbol k ->
+    option (Finnat number_of_states * symbol k * direction);
+  start_state : Finnat number_of_states
 }.
+Arguments number_of_states {k}.
+Arguments transition_function {k}.
+Arguments start_state {k}.
 
-Record Tape (tm : TM) : Set := make_tape {
+Definition state {k : nat} (tm : TM k) : Set := Finnat (number_of_states tm).
+
+Record Config {k : nat} (tm : TM k) : Set := makeConfig {
   cur_state : state tm;
-  tape_left : list (symbol tm);      
-  current_symbol : symbol tm;       
-  tape_right : list (symbol tm)     
+  tape_left : list (symbol k);   (* cell at head-1 is the list head *)
+  current_symbol : symbol k;
+  tape_right : list (symbol k)   (* cell at head+1 is the list head *)
 }.
-Arguments make_tape {tm}.
-Arguments cur_state {tm}.
-Arguments tape_left {tm}.
-Arguments current_symbol {tm}.
-Arguments tape_right {tm}.
+Arguments makeConfig {k tm}.
+Arguments cur_state {k tm}.
+Arguments tape_left {k tm}.
+Arguments current_symbol {k tm}.
+Arguments tape_right {k tm}.
 
+Definition init {k : nat} (tm : TM k) : Config tm :=
+  makeConfig (start_state tm) [] blank [].
 
-Definition init (tm : TM) : Tape tm :=
-  make_tape (start_state tm) [] (blank_symbol tm) [].
-
-Definition halts (tm : TM) (config : Tape tm) : bool :=
-  match transition_function tm (cur_state config) (current_symbol config) with
+Definition halts {k : nat} (tm : TM k) (c : Config tm) : bool :=
+  match transition_function tm (cur_state c) (current_symbol c) with
   | None => true
   | Some _ => false
   end.
 
-Definition step (tm : TM) (config : Tape tm) : option (Tape tm) :=
-  match transition_function tm (cur_state config) (current_symbol config) with
+Definition step {k : nat} (tm : TM k) (c : Config tm) : option (Config tm) :=
+  match transition_function tm (cur_state c) (current_symbol c) with
   | None => None
   | Some (s', sym', d) =>
       match d with
       | L =>
-          let new_current := match tape_left config with
-                             | [] => blank_symbol tm
+          let new_current := match tape_left c with
+                             | [] => blank
                              | h :: _ => h
                              end in
-          let new_left := match tape_left config with
+          let new_left := match tape_left c with
                           | [] => []
                           | _ :: t => t
                           end in
-          let new_right := sym' :: tape_right config in
-          Some (make_tape s' new_left new_current new_right)
+          Some (makeConfig s' new_left new_current (sym' :: tape_right c))
       | R =>
-          let new_current := match tape_right config with
-                             | [] => blank_symbol tm
+          let new_current := match tape_right c with
+                             | [] => blank
                              | h :: _ => h
                              end in
-          let new_right := match tape_right config with
+          let new_right := match tape_right c with
                            | [] => []
                            | _ :: t => t
                            end in
-          let new_left := sym' :: tape_left config in
-          Some (make_tape s' new_left new_current new_right)
+          Some (makeConfig s' (sym' :: tape_left c) new_current new_right)
       end
   end.
 
-Fixpoint run_steps (tm : TM) (config : Tape tm) (n : nat) : option (Tape tm) :=
+Fixpoint run_steps {k : nat} (tm : TM k) (c : Config tm) (n : nat)
+  : option (Config tm) :=
   match n with
-  | O => Some config
-  | S n' => match run_steps tm config n' with
-            | Some config' => step tm config'
+  | O => Some c
+  | S n' => match run_steps tm c n' with
+            | Some c' => step tm c'
             | None => None
             end
   end.
-(* TM with config c1 visits config c2 in n steps *)
-Definition run (tm : TM) (c1 c2 : Tape tm) : Prop :=
-  exists n, run_steps tm c1 n = Some c2.
-(* TM halts after n steps *)
-Definition takes_steps (tm : TM) (start : Tape tm) (n : nat) : Prop :=
-  exists config, run_steps tm start n = Some config /\ halts tm config = true.
 
-(* For all step numbers n, TM with given config does not halt. *)
-Definition runs_forever (tm : TM) (start : Tape tm) : Prop :=
-  forall n, exists config, run_steps tm start n = Some config.
+(* tm, started in c1, is in configuration c2 after n steps *)
+Definition run {k : nat} (tm : TM k) (c1 c2 : Config tm) (n : nat) : Prop :=
+  run_steps tm c1 n = Some c2.
+
+Lemma run_steps_deterministic {k : nat} (tm : TM k) (c c1 c2 : Config tm) (n : nat) :
+  run_steps tm c n = Some c1 -> run_steps tm c n = Some c2 -> c1 = c2.
+Proof. congruence. Qed.
+
+Lemma halts_step {k : nat} (tm : TM k) (c : Config tm) :
+  halts tm c = true -> step tm c = None.
+Proof.
+  unfold halts, step.
+  destruct (transition_function tm (cur_state c) (current_symbol c))
+    as [[[s' sym'] d]|]. discriminate.  reflexivity.
+Qed.
+(* Addition of steps is associative. *)
+Lemma run_steps_plus {k : nat} (tm : TM k) (c : Config tm) (a b : nat) :
+  run_steps tm c (a + b) =
+  match run_steps tm c b with
+  | Some c' => run_steps tm c' a
+  | None => None
+  end.
+Proof.
+  induction a as [|a IH]; simpl.
+  - destruct (run_steps tm c b); reflexivity.
+  - rewrite IH. destruct (run_steps tm c b) as [c'|]; reflexivity.
+Qed.
+
+(* Addition of steps after halting is idempotent: f∘f=f *)
+Lemma run_steps_halted {k : nat} (tm : TM k) (c : Config tm) (n : nat) :
+  halts tm c = true -> run_steps tm c (S n) = None.
+Proof.
+  intros H. induction n as [|n IH]; simpl.
+  - rewrite halts_step. reflexivity. rewrite H. reflexivity.
+  - simpl in IH.  rewrite IH. reflexivity.
+ Qed.
+
+(*For a given tape configuration, halting state and tape is unique. *)
+Lemma halting_unique {k : nat} (tm : TM k) (c : Config tm)
+    (n1 n2 : nat) (c1 c2 : Config tm) :
+  run_steps tm c n1 = Some c1 -> halts tm c1 = true ->
+  run_steps tm c n2 = Some c2 -> halts tm c2 = true ->
+  c1 = c2.
+Proof.
+  intros Hrun1 Hhalt1 Hrun2 Hhalt2.
+  (* trichotomy destructs c1=c2 to cases <, >, = *)
+  destruct (Nat.lt_trichotomy n1 n2) as [Hlt | [Heq | Hgt]].
+  - (* n1 < n2 *)
+    exfalso.
+    assert (Hsplit : n2 = (n2 - n1) + n1) by lia.
+    rewrite Hsplit in Hrun2.
+    rewrite run_steps_plus in Hrun2.
+    rewrite Hrun1 in Hrun2.
+    destruct (n2 - n1) as [|m].
+    + lia.
+    + rewrite run_steps_halted in Hrun2 by exact Hhalt1.
+      discriminate.
+  - (* n1 = n2 *)
+    subst.
+    rewrite Hrun1 in Hrun2. injection Hrun2 as ->.  reflexivity.
+  - (* n2 < n1 *)
+    exfalso.
+    assert (Hsplit : n1 = (n1 - n2) + n2) by lia.
+    rewrite Hsplit in Hrun1.
+    rewrite run_steps_plus in Hrun1.
+    rewrite Hrun2 in Hrun1.
+    destruct (n1 - n2) as [|m].
+    + lia.
+    + rewrite run_steps_halted in Hrun1 by exact  Hhalt2.
+      discriminate.
+Qed.
 
 
-Definition is_non_blank {tm : TM} (s : symbol tm) : bool :=
-  if Fin.eq_dec s (blank_symbol tm) then false else true.
-  
+Definition is_non_blank {k : nat} (s : symbol k) : bool :=
+  if Finnat_eq_dec s blank then false else true.
 
-Fixpoint count_non_blank_list {tm : TM} (l : list (symbol tm)) : nat :=
+Fixpoint count_non_blank_list {k : nat} (l : list (symbol k)) : nat :=
   match l with
   | [] => O
-  | h :: t => if is_non_blank h then S (count_non_blank_list t) else count_non_blank_list t
+  | h :: t => if is_non_blank h
+              then S (count_non_blank_list t)
+              else count_non_blank_list t
   end.
 
-Definition count_non_blank_state {tm : TM} (config : Tape tm) : nat :=
-  count_non_blank_list (tape_left config) +
-  (if is_non_blank (current_symbol config) then 1 else 0) +
-  count_non_blank_list (tape_right config).
+Definition count_non_blank {k : nat} {tm : TM k} (c : Config tm) : nat :=
+  count_non_blank_list (tape_left c) +
+  (if is_non_blank (current_symbol c) then 1 else 0) +
+  count_non_blank_list (tape_right c).
 
-(* Definition for a TM producing m non-blank symbols upon halting *)
-Definition produces_ones (tm : TM) (m : nat) : Prop :=
-  exists (steps : nat) (config : Tape tm),
-    run_steps tm (init tm) steps = Some config /\
-    halts tm config = true /\
-    count_non_blank_state config = m.
+(* tm, started on the blank tape, halts with m non-blank symbols. *)
+Definition BB_score {k : nat} (tm : TM k) (m : nat) : Prop :=
+  exists (n : nat) (c : Config tm),
+    run_steps tm (init tm) n = Some c /\
+    halts tm c = true /\
+    count_non_blank c = m.
 
-(* Busy Beaver Sigma Function BB(n) *)
-Definition BB (n ones : nat) : Prop :=
-  (* There exists a TM with n states and 2 symbols that produces ones non-blank symbols upon halting *)
-  (exists tm : TM,
-     number_of_states tm = n /\
-     number_of_symbols tm = 2%nat /\
-     produces_ones tm ones)
+(* BB n m: some n-state 2-symbol machine achieves m, and none exceeds it. *)
+Definition BB (n m : nat) : Prop :=
+  (exists tm : TM 0,
+      number_of_states tm = n /\ BB_score tm m)
   /\
-  (* and this TM scores the highest number of ones before halting *)
-  (forall tm : TM,
-     number_of_states tm = n ->
-     number_of_symbols tm = 2%nat ->
-     forall m, produces_ones tm m -> (m <= ones)%nat).
+  (forall (tm : TM 0) (m' : nat),
+      number_of_states tm = n -> BB_score tm m' -> m' <= m).
 
-(* A TM that runs forever *)
-Definition loop_tm : TM := {|
-  number_of_states := 1; number_of_symbols := 2;
-  blank_symbol := Fin.F1;
-  transition_function := fun s sym => Some (s, sym , R);
-  start_state := Fin.F1
-|}.
+Lemma BB_functional (n m1 m2 : nat) :
+  BB n m1 -> BB n m2 -> m1 = m2.
+Proof.
+  intros [(tm1 & Hstates1 & Hscore1) Hmax1]
+         [(tm2 & Hstates2 & Hscore2) Hmax2].
+  specialize (Hmax2 tm1 m1 Hstates1 Hscore1). (* m1 <= m2 *)
+  specialize (Hmax1 tm2 m2 Hstates2 Hscore2). (* m2 <= m1 *)
+  lia. 
+Qed.
+(* Partial is not necessarily defined for all elements in the domain, e.g. f(n)=m iff m^2 = n, m ∈ N , n ∈ Z *)
+(* A partial function is not necessarily total. Busy Beaver is a total function. *)
+Record partfun (A B : Type) : Type := mkPartfun {
+  funrel :> A -> B -> Prop;
+  (* A funrel must be deterministic: f(x) = y1 -> f(x) = y2  -> y1 = y2 *)
+  functional : forall x y1 y2, funrel x y1 -> funrel x y2 -> y1 = y2
+}.
+Arguments funrel {A B}.
+Arguments functional {A B}.
+(* Every total function is also a partial function. *)
+Definition partfun_of_fun {A B : Type} (f : A -> B) : partfun A B.
+Proof.
+  refine {| funrel := fun x y => f x = y |}.
+  intros x y1 y2 H1 H2. subst. reflexivity. 
+Defined.
+(* equality of partial functions *)
+Definition partfun_eq {A B : Type} (f1 f2 : partfun A B) : Prop :=
+  forall x y, funrel f1 x y <-> funrel f2 x y.
 
+Definition BB_pf : partfun nat nat :=
+  {| funrel := BB; functional := BB_functional |}.
 
-Compute run_steps loop_tm (init loop_tm) 5.  
-Compute halts loop_tm (init loop_tm).       
- 
-(* A TM that halts immediately *)
-Definition halt_tm : TM := {|
-  number_of_states := 1; number_of_symbols := 2;
-  blank_symbol := Fin.F1;
-  transition_function := fun s sym => None;
-  start_state := Fin.F1
-|}.
+  (* Value of BB is encoding where head points the leftmost of the tape and unary marks are lined up to the right *)
+Definition encoding_config {k : nat} (tm : TM k) (n : nat) : Config tm :=
+  match n with
+  | O => init tm
+  | S n' => makeConfig (start_state tm) [] one (repeat one n')
+  end.
 
-Compute run_steps halt_tm (init halt_tm) 0.
-Compute run_steps halt_tm (init halt_tm) 10.  
+(* l consists of n marks followed by blanks. *)
+Definition encodes_list {k : nat} (l : list (symbol k)) (n : nat) : Prop :=
+  exists prefix suffix,
+    l = prefix ++ suffix /\
+    length prefix = n /\
+    Forall (fun x => x = one) prefix /\
+    Forall (fun x => x = blank) suffix.
 
-(* Unary encoding of natural numbers *)
-Definition encodes {tm : TM} (config : Tape tm) (n : nat) : Prop :=
-  exists s : symbol tm,
-    s <> blank_symbol tm /\
-    Forall (fun x => x = blank_symbol tm) (tape_left config) /\ (* left of tape is blank *)
-     (* if n is zero, tape is blank else construct prefix as a sequence of s *)
-    match n with
-    | O => current_symbol config = blank_symbol tm /\ Forall (fun x => x = blank_symbol tm) (tape_right config)
-    | S n' =>
-        current_symbol config = s /\
-        (* prefix = n' and  suffix = [blank_symbol tm]*)
-        exists prefix suffix,
-          tape_right config = prefix ++ suffix /\
-          length prefix = n' /\
-          Forall (fun x => x = s) prefix /\
-          Forall (fun x => x = blank_symbol tm) suffix
-    end.
-(* A TM M is said to compute a function f:Σ*↦Σ* iff M halts and encodes f(n) *)
-Definition computes_function (tm : TM) (f : nat -> nat -> Prop) : Prop :=
-  exists mark : symbol tm,
-    mark <> blank_symbol tm /\
-    forall n m : nat, f n m ->
-      exists config : Tape tm,
-        run tm (init tm) config /\
-        halts tm config = true /\
-        encodes config m.
+Definition encodes {k : nat} {tm : TM k} (c : Config tm) (n : nat) : Prop :=
+  Forall (fun x => x = blank) (tape_left c) /\
+  encodes_list (current_symbol c :: tape_right c) n.
 
-Proposition BB_uncomputable : ~exists tm : TM, computes_function tm BB.
-Admitted.
+(* A list of marks that is also a list of blanks is empty. *)
+Lemma all_one_all_blank_nil {k : nat} (l : list (symbol k)) :
+  Forall (fun x => x = one) l -> Forall (fun x => x = blank) l -> l = [].
+Proof.
+  intros H1 H2. destruct l as [|h t]. reflexivity.
+  inversion H1. inversion H2. subst.
+  exfalso. apply (@blank_neq_one k). congruence.
+Qed.
+
+Lemma encodes_list_functional {k : nat} (l : list (symbol k)) (n1 n2 : nat) :
+  encodes_list l n1 -> encodes_list l n2 -> n1 = n2.
+Proof.
+  intros (p1 & s1 & Hl1 & Hlen1 & Hone1 & Hblank1)
+         (p2 & s2 & Hl2 & Hlen2 & Hone2 & Hblank2).
+  subst n1 n2.
+  assert (Hpp : p1 ++ s1 = p2 ++ s2) by congruence.
+  destruct (app_eq_app _ _ _ _ Hpp) as (m & [[Hp Hs] | [Hp Hs]]); subst.
+  - (* p1 = p2 ++ m, s2 = m ++ s1 : m is all-one and all-blank, so [] *)
+    apply Forall_app in Hone1 as [_ Hm1].
+    apply Forall_app in Hblank2 as [Hm2 _].
+    rewrite (all_one_all_blank_nil m Hm1 Hm2). rewrite app_nil_r. reflexivity.
+  - (* p2 = p1 ++ m, s1 = m ++ s2 : symmetric *)
+    apply Forall_app in Hone2 as [_ Hm1].
+    apply Forall_app in Hblank1 as [Hm2 _].
+    rewrite (all_one_all_blank_nil m Hm1 Hm2). rewrite app_nil_r. reflexivity.
+Qed.
+
+Lemma encodes_functional {k : nat} {tm : TM k} (c : Config tm) (m1 m2 : nat) :
+  encodes c m1 -> encodes c m2 -> m1 = m2.
+Proof.
+  (* eapply creates existential variable ?l*)
+  (*eauto : Implements a Prolog-like resolution procedure to solve the current goal.
+   It first tries to solve the goal using the assumption tactic, 
+   then it reduces the goal to an atomic one using intros and introduces the newly generated hypotheses as hints.
+    Then it looks at the list of tactics associated with the head symbol of the goal and tries to apply one of them. 
+  Lower cost tactics are tried before higher-cost tactics. This process is recursively applied to the generated subgoals.*)
+  intros [_ H1] [_ H2]. eapply encodes_list_functional. eauto. eauto.
+Qed.
+
+(* On input n, tm halts with output m  *)
+Definition computes {k : nat} (tm : TM k) (n m : nat) : Prop :=
+  exists (steps : nat) (c : Config tm),
+    run_steps tm (encoding_config tm n) steps = Some c /\
+    halts tm c = true /\
+    encodes c m.
+
+Lemma computes_functional {k : nat} (tm : TM k) (n m1 m2 : nat) :
+  computes tm n m1 -> computes tm n m2 -> m1 = m2.
+Proof.
+  (*st1: # of steps for tm1, i.e. n*)
+  intros (st1 & c1 & Hr1 & Hh1 & He1) (st2 & c2 & Hr2 & Hh2 & He2).
+  assert (c1 = c2). eapply halting_unique. eauto. eauto. eauto. eauto.   subst.
+  eapply encodes_functional. eauto. eauto.
+Qed.
+
+Definition computes_pf {k : nat} (tm : TM k) : partfun nat nat :=
+  {| funrel := computes tm; functional := computes_functional tm |}.
+(* A function is computable iff there exists some Turing machine that computes it *)
+Definition computable (f : nat -> nat -> Prop) : Prop :=
+  exists tm : TM 0,
+    forall n m, f n m <-> computes tm n m.
+
+(* left embedding :  s < n1 + n2 *)
+Lemma embed_l_lt {n1 : nat} (n2 : nat) (s : Finnat n1) :
+  finnat_val s < n1 + n2.
+Proof. destruct s. simpl. lia. Qed.
+
+Definition embed_l {n1 : nat} (n2 : nat) (s : Finnat n1) : Finnat (n1 + n2) :=
+  {| finnat_val := s; finnat_lt := embed_l_lt n2 s |}.
+
+Lemma embed_r_lt (n1 : nat) {n2 : nat} (s : Finnat n2) :
+   n1 + finnat_val s < n1 + n2.
+Proof. destruct s. simpl. lia. Qed.
+
+Definition embed_r (n1 : nat) {n2 : nat} (s : Finnat n2) : Finnat (n1 + n2) :=
+  {| finnat_val := n1 + s; finnat_lt := embed_r_lt n1 s |}.
+
+Lemma split_lt (n1 n2 v : nat) : v < n1 + n2 -> ~ v < n1 -> v - n1 < n2.
+Proof. lia. Qed.
+
+(* Split a state of the combined machine into tm1's side or tm2's side. *)
+Definition split_fin (n1 n2 : nat) (s : Finnat (n1 + n2))
+  : Finnat n1 + Finnat n2 :=
+  match lt_dec s n1 with
+  (* if s < n1, s belongs to tm1 *)
+  | left H => inl {| finnat_val := s; finnat_lt := H |}
+  (* if s >= n1, s belongs to tm2 *)
+  | right H => inr {| finnat_val := finnat_val s - n1;
+                      finnat_lt := split_lt n1 n2 _ (finnat_lt s) H |}
+  end.
+
+Lemma split_fin_embed_l (n1 n2 : nat) (s : Finnat n1) :
+  split_fin n1 n2 (embed_l n2 s) = inl s.
+Proof.
+  unfold split_fin. simpl.
+  destruct (lt_dec (finnat_val s) n1).
+  - f_equal. apply Finnat_ext. reflexivity.
+  - exfalso. destruct s. simpl in *. lia.
+Qed.
+
+Lemma split_fin_embed_r (n1 n2 : nat) (s : Finnat n2) :
+  split_fin n1 n2 (embed_r n1 s) = inr s.
+Proof.
+  unfold split_fin. simpl.
+  destruct (lt_dec (n1 + finnat_val s) n1) as [H | H].
+  - exfalso. lia.
+  - f_equal. apply Finnat_ext. simpl. lia.
+Qed.
+
+(* M.N: run M; if and when M halts, pass control to N on the same tape.  *)
+Definition compose {k : nat} (tm1 tm2 : TM k) : TM k :=
+  {| number_of_states := number_of_states tm1 + number_of_states tm2;
+     start_state := embed_l (number_of_states tm2) (start_state tm1);
+     transition_function := fun s sym =>
+       match split_fin _ _ s with
+       (*tm1*)
+       | inl s1 =>
+           match transition_function tm1 s1 sym with
+           (* tm1 has a transition *)
+           | Some (s1', sym', d) => Some (embed_l (number_of_states tm2) s1', sym', d)
+           (* tm1 halts tm2 begins*)
+           | None =>
+               match transition_function tm2 (start_state tm2) sym with
+               (* tm2 has a transition *)
+               | Some (s2', sym', d) => Some (embed_r (number_of_states tm1) s2', sym', d)
+               (* tm2 has no transition, halts *)
+               | None => None
+               end
+           end
+       | inr s2 =>
+           match transition_function tm2 s2 sym with
+            (* tm2 has a transition *)
+           | Some (s2', sym', d) => Some (embed_r (number_of_states tm1) s2', sym', d)
+           (* tm2 has no transition, halts *)
+           | None => None
+           end
+       end |}.
+
+Lemma compose_states {k : nat} (tm1 tm2 : TM k) :
+  number_of_states (compose tm1 tm2)
+  = number_of_states tm1 + number_of_states tm2.
+Proof. reflexivity. Qed.
+
+Definition lift_l {k : nat} {tm1 tm2 : TM k} (c : Config tm1)
+  : Config (compose tm1 tm2) :=
+  makeConfig (tm := compose tm1 tm2)
+           (embed_l (number_of_states tm2) (cur_state c))
+           (tape_left c) (current_symbol c) (tape_right c).
+
+Definition lift_r {k : nat} {tm1 tm2 : TM k} (c : Config tm2)
+  : Config (compose tm1 tm2) :=
+  makeConfig (tm := compose tm1 tm2)
+           (embed_r (number_of_states tm1) (cur_state c))
+           (tape_left c) (current_symbol c) (tape_right c).
